Some more progress on making the unifier nicely executable

type_checker/unifyScript.sml
@@ -15,6 +15,14 @@ val FMAP2_FMAP2 = Q.prove (
 ho_match_mp_tac fmap_INDUCT >>
 rw [FMAP_MAP2_FEMPTY, FMAP_MAP2_FUPDATE]);
 
+val option_bind_thm = Q.prove (
+`!x f. OPTION_BIND x f =
+  case x of
+    | NONE => NONE
+    | SOME y => f y`,
+cases_on `x` >>
+rw [OPTION_BIND_def]);
+
 val _ = new_theory "unify";
 
 val _ = Hol_datatype `
@@ -92,7 +100,7 @@ rw [FLOOKUP_FMAP2, option_map_def, encode_infer_t_def]);
 
 val t_vwalk_ind = save_thm("t_vwalk_ind", (UNDISCH o Q.SPEC `s`) t_vwalk_ind')
 
-val t_vwalk_eqns = Q.store_thm ("t_vwalk_eqns",
+val t_vwalk_eqn = Q.store_thm ("t_vwalk_eqn",
 `!s. 
   t_wfs s ⇒
   (!v. 
@@ -103,8 +111,6 @@ val t_vwalk_eqns = Q.store_thm ("t_vwalk_eqns",
       | SOME (Infer_Tfn t1 t2) => Infer_Tfn t1 t2
       | SOME (Infer_Tapp ts tc') => Infer_Tapp ts tc'
       | SOME (Infer_Tvar_db n) => Infer_Tvar_db n)`,
-NTAC 2 STRIP_TAC >>
-ho_match_mp_tac t_vwalk_ind >>
 rw [t_vwalk_def] >>
 full_case_tac >>
 rw [] >>
@@ -122,7 +128,7 @@ fs [t_wfs_def] >|
 val t_walk_def = Define `
 t_walk s t = decode_infer_t (walk (FMAP_MAP2 (\(n,t). encode_infer_t t) s) (encode_infer_t t))`;
 
-val t_walk_eqns = Q.store_thm ("t_walk_eqns",
+val t_walk_eqn = Q.store_thm ("t_walk_eqn",
 `(!s v. t_walk s (Infer_Tuvar v) = t_vwalk s v) ∧
  (!s t1 t2. t_walk s (Infer_Tfn t1 t2) = Infer_Tfn t1 t2) ∧
  (!s ts tc. t_walk s (Infer_Tapp ts tc) = Infer_Tapp ts tc) ∧
@@ -133,21 +139,9 @@ rw [t_walk_def, walk_def, t_vwalk_def, encode_infer_t_def,
 val t_oc_def = Define `
 t_oc s t v = oc (FMAP_MAP2 (\(n,t). encode_infer_t t) s) (encode_infer_t t) v`;
 
+(*
 val t_vars_def = Define `
 t_vars t = vars (encode_infer_t t)`;
-
-val encode_vwalk = Q.prove (
-`!s. t_wfs s ⇒ !u. vwalk (FMAP_MAP2 (λ(n,t). encode_infer_t t) s) u = encode_infer_t (t_vwalk s u)`,
-NTAC 2 STRIP_TAC >>
-ho_match_mp_tac t_vwalk_ind >>
-rw [] >>
-`wfs (FMAP_MAP2 (\(n,t). encode_infer_t t) s)` by metis_tac [t_wfs_def] >>
-rw [Once vwalk_def] >>
-rw [Once t_vwalk_eqns, FLOOKUP_FMAP2] >>
-cases_on `FLOOKUP s u` >>
-rw [option_map_def, encode_infer_t_def] >>
-cases_on `x` >>
-rw [encode_infer_t_def]);
 
 val t_oc_ind' = Q.prove (
 `∀s oc'.
@@ -175,23 +169,44 @@ val t_oc_ind = Q.store_thm ("t_oc_ind",
   (∀a0 a1. t_oc s a0 a1 ⇒ oc' a0 a1)`,
 rw [t_oc_def] >>
 metis_tac [t_oc_ind', FMAP2_FMAP2, FMAP2_id, decode_left_inverse]);
+*)
 
-(*
-val t_oc_eqns' = Q.prove
+val encode_vwalk = Q.prove (
+`!s. t_wfs s ⇒ !u. vwalk (FMAP_MAP2 (λ(n,t). encode_infer_t t) s) u = encode_infer_t (t_vwalk s u)`,
+NTAC 2 STRIP_TAC >>
+ho_match_mp_tac t_vwalk_ind >>
+rw [] >>
+`wfs (FMAP_MAP2 (\(n,t). encode_infer_t t) s)` by metis_tac [t_wfs_def] >>
+rw [Once vwalk_def] >>
+rw [Once t_vwalk_eqn, FLOOKUP_FMAP2] >>
+cases_on `FLOOKUP s u` >>
+rw [option_map_def, encode_infer_t_def] >>
+cases_on `x` >>
+rw [encode_infer_t_def]);
+
+val t_oc_eqn_help = Q.prove (
+`!l v s.
+  oc (FMAP_MAP2 (λ(n,t). encode_infer_t t) s) (encode_infer_ts l) v ⇔
+  EXISTS (λt. oc (FMAP_MAP2 (λ(n,t). encode_infer_t t) s) (encode_infer_t t) v) l`,
+induct_on `l` >>
+rw [encode_infer_t_def]);
+
+val t_oc_eqn = Q.store_thm ("t_oc_eqn",
 `!s. t_wfs s ⇒
-  !t v. t_oc s t v ⇒
+  !t v. t_oc s t v =
     case t_walk s t of
       | Infer_Tuvar u => v = u
       | Infer_Tfn t1 t2 => t_oc s t1 v ∨ t_oc s t2 v
       | Infer_Tapp ts tc' => EXISTS (\t. t_oc s t v) ts
       | Infer_Tvar_db n => F`,
-NTAC 2 STRIP_TAC >>
-ho_match_mp_tac t_oc_ind >>
-rw [] >>
+rw [t_oc_def] >>
+`wfs (FMAP_MAP2 (λ(n,t). encode_infer_t t) s)` by fs [t_wfs_def] >>
+rw [Once oc_walking, t_walk_def] >>
 cases_on `t` >>
-rw [t_walk_eqns] >>
-fs [t_vars_def, encode_infer_t_def]
-*)
+rw [walk_def, encode_infer_t_def, decode_infer_t_def, decode_left_inverse,
+    encode_vwalk, t_oc_eqn_help] >>
+cases_on `t_vwalk s n` >>
+rw [encode_infer_t_def, t_oc_eqn_help]);
 
 val t_ext_s_check_def = Define `
 t_ext_s_check s v t =
@@ -199,7 +214,7 @@ t_ext_s_check s v t =
     (FMAP_MAP2 (\(n,t). decode_infer_t t))
     (ext_s_check (FMAP_MAP2 (\(n,t). encode_infer_t t) s) v (encode_infer_t t))`;
 
-val t_ext_s_check_eqns = Q.store_thm ("t_ext_s_check_eqns",
+val t_ext_s_check_eqn = Q.store_thm ("t_ext_s_check_eqn",
 `!s v t.
   t_ext_s_check s v t = if t_oc s t v then NONE else SOME (s |+ (v,t))`,
 rw [t_ext_s_check_def, t_oc_def, option_map_def, FMAP_MAP2_FUPDATE, 
@@ -216,25 +231,69 @@ val ts_unify_def = Define `
 (ts_unify s (t1::ts1) (t2::ts2) =
   case t_unify s t1 t2 of
    | NONE => NONE
-   | SOME s' => ts_unify s' ts1 ts2)`;
-
-   (*
-val t_unify_ind = Q.store_thm ("t_unify_ind",
-`∀P.
-  (∀s t1 t2.
-    (∀t1a t1d t2a t2d sx.
-      t_wfs s ∧ (t_walk s t1 = Pair t1a t1d) ∧
-      (t_walk s t2 = Pair t2a t2d) ∧ (t_unify s t1a t2a = SOME sx) ⇒
-      P sx t1d t2d) ∧
-    (∀t1a t1d t2a t2d.
-      t_wfs s ∧ (t_walk s t1 = Pair t1a t1d) ∧
-      (t_walk s t2 = Pair t2a t2d) ⇒
-      P s t1a t2a) ⇒
-    P s t1 t2) ⇒
-  ∀v v1 v2. P v v1 v2`,
+   | SOME s' => ts_unify s' ts1 ts2) ∧
+(ts_unify s _ _ = NONE)`;
 
 
+val encode_unify = Q.prove (
+`!s t1 t2 s' t1' t2'.
+  (s = (FMAP_MAP2 (λ(n,t). encode_infer_t t) s')) ∧
+  (t1 = encode_infer_t t1') ∧ 
+  (t2 = encode_infer_t t2') ∧ 
+  t_wfs s' ⇒
+  (unify s t1 t2
+   =
+   option_map (FMAP_MAP2 (λ(n,t). encode_infer_t t)) (t_unify s' t1' t2'))`,
+ho_match_mp_tac unify_ind >>
+rw [t_unify_def] >>
+cases_on `unify (FMAP_MAP2 (λ(n,t). encode_infer_t t) s') (encode_infer_t t1') (encode_infer_t t2')` >>
+rw [option_map_def, FMAP2_FMAP2, decode_left_inverse, FMAP2_id] >>
+cases_on `t1'` >>
+cases_on `t2'` >>
+fs [walk_def, encode_infer_t_def] >>
+`wfs (FMAP_MAP2 (λ(n,t). encode_infer_t t) s')` by metis_tac [t_wfs_def] >>
+fs [Once unify_def] >>
+rw [option_map_def, FMAP2_FMAP2, decode_left_inverse, FMAP2_id, encode_vwalk] >>
+cheat);
 
+val wfs_unify = Q.prove (
+`!s t1 t2 s'. (unify s t1 t2 = SOME s') ⇒ wfs s'`,
+cheat);
+
+val ts_unify_thm = Q.prove (
+`!s l1 l2.
+  t_wfs s ⇒
+  (ts_unify s l1 l2 =
+   option_map (FMAP_MAP2 (λ(n,t). decode_infer_t t))
+     (unify (FMAP_MAP2 (λ(n,t). encode_infer_t t) s) (encode_infer_ts l1) (encode_infer_ts l2)))`,
+induct_on `l1` >>
+cases_on `l2` >>
+rw [ts_unify_def, encode_infer_t_def] >>
+`wfs (FMAP_MAP2 (\(n,t). encode_infer_t t) s)` by metis_tac [t_wfs_def] >|
+[rw [Once unify_def, option_map_def, decode_left_inverse, FMAP2_FMAP2, FMAP2_id],
+ rw [Once unify_def, option_map_def, ts_unify_def],
+ rw [Once unify_def, option_map_def, ts_unify_def],
+ rw [Once unify_def] >>
+     cases_on `t_unify s h' h` >>
+     rw [] >|
+     [fs [t_unify_def, option_bind_thm] >>
+          every_case_tac >>
+          fs [option_map_def],
+      fs [t_unify_def, option_bind_thm] >>
+          every_case_tac >>
+          fs [option_map_def] >>
+          rw [FMAP2_FMAP2, FMAP2_id] >>
+          `?x. x' = FMAP_MAP2 (λ(n,t). encode_infer_t t) x`
+                by (imp_res_tac encode_unify >>
+                    fs [option_map_def] >>
+                    cases_on `t_unify s h' h` >>
+                    fs [] >>
+                    metis_tac []) >>
+          `t_wfs x` by
+                 (rw [t_wfs_def] >>
+                  metis_tac [wfs_unify]) >>
+          rw [FMAP2_FMAP2, FMAP2_id, decode_left_inverse]]]);
+(*
 val t_unify_eqn = Q.store_thm ("t_unify_eqn",
 `(!t1 t2 s.
   t_wfs s ⇒
@@ -258,34 +317,62 @@ val t_unify_eqn = Q.store_thm ("t_unify_eqn",
           SOME s 
         else
           NONE
-    | _ => NONE)) ∧
- (!ts1 ts2 s.
-  t_wfs s ⇒
-  (ts_unify s ts1 ts2 = ts_unify s ts1 ts2))`, 
+    | _ => NONE))`,
 
-ho_match_mp_tac infer_t_induction >>
-rw [] >>
-cases_on `t2` >>
-rw [encode_infer_t_def, t_unify_def, t_walk_eqns] >>
+rw [t_unify_def] >>
 `wfs (FMAP_MAP2 (\(n,t). encode_infer_t t) s)` by metis_tac [t_wfs_def] >>
-rw [Once unify_def, option_map_def] >|
-[rw [FMAP2_FMAP2, decode_left_inverse, FMAP2_id],
- rw [Once t_vwalk_eqns, Once vwalk_def, FLOOKUP_FMAP2] >>
-     cases_on `FLOOKUP s n'` >>
-     rw [option_map_def] >|
-     [all_tac,
-      cases_on `x` >>
-          rw [encode_infer_t_def] >|
-          [all_tac,
-           
-           
-     
-     
-     , FMAP_MAP2_FUPDATE, decode_left_inverse, FMAP2_id, FMAP2_FMAP2,
-         decode_infer_t_def]
+rw [Once unify_def, t_walk_def] >>
+cases_on `t1` >>
+cases_on `t2` >>
+rw [encode_infer_t_def, decode_infer_t_def, option_map_def, decode_left_inverse,
+    FMAP2_FMAP2, FMAP2_id, encode_vwalk, option_bind_thm] >|
+[cases_on `t_vwalk s n'` >>
+     rw [encode_infer_t_def, option_map_def, FMAP2_FMAP2, decode_left_inverse,
+         FMAP2_id, FMAP_MAP2_FUPDATE, decode_infer_t_def] >>
+     rw [t_ext_s_check_eqn] >>
+     imp_res_tac t_oc_eqn >>
+     pop_assum (fn x => ALL_TAC) >>
+     pop_assum (fn x => ALL_TAC) >>
+     pop_assum (ASSUME_TAC o Q.SPECL [`n''`, `Infer_Tvar_db n`]) >>
+     fs [] >>
+     rw [t_walk_def, encode_infer_t_def, decode_infer_t_def],
+ rw [Once unify_def] >>
+     rw [Once unify_def] >>
+     rw [Once unify_def] >>
+     rw [ts_unify_thm, option_map_def],
+ rw [Once unify_def] >>
+     rw [Once unify_def] >>
+     rw [Once unify_def],
+ rw [Once unify_def],
+ cases_on `t_vwalk s n` >>
+     rw [encode_infer_t_def] >>
+     rw [Once unify_def] >>
+     rw [Once unify_def] >>
+     rw [Once unify_def] >>
+     rw [ts_unify_thm, option_map_def, FMAP2_FMAP2, decode_left_inverse,
+         FMAP2_id, FMAP_MAP2_FUPDATE, decode_infer_t_def, t_ext_s_check_eqn, option_map_def] >>
+     rw [Once oc_walking, encode_infer_t_def, t_oc_def],
+ rw [Once unify_def],
+ rw [Once unify_def] >>
+     rw [Once unify_def] >>
+     cases_on `unify (FMAP_MAP2 (λ(n,t). encode_infer_t t) s) (encode_infer_t i) (encode_infer_t i')` >>
+     fs [] >>
+     cases_on `unify x (encode_infer_t i0) (encode_infer_t i0')` >>
+     fs [] >>
+     `?x'. x = FMAP_MAP2 (λ(n,t). encode_infer_t t) x'`
+           by (imp_res_tac encode_unify >>
+               fs [option_map_def] >>
+               cases_on `t_unify s i i'` >>
+               fs [] >>
+               metis_tac []) >>
+    rw [FMAP2_FMAP2, FMAP2_id, decode_left_inverse],
+ all_tac,
+ all_tac,
+ all_tac,
+ all_tac,
+ all_tac]
 
-         *)
-
+ *) 
 
 val apply_subst_t = Define `
 apply_subst_t s t = decode_infer_t (subst_APPLY (FMAP_MAP2 (\(n,t). encode_infer_t t) s) (encode_infer_t t))`;
